Looking at state, only monotonicity

state/experiments/ComputationalView.fst
@@ -12,7 +12,6 @@ let pure_wp_bind (m:pure_wp 'a) (k:'a -> pure_wp 'b) : pure_wp 'b =
 let pure_wp_stronger (wp1 wp2:pure_wp 'a) : Type0 =
   forall p. wp2 p ==> wp1 p
 
-
 let rec freePure_theta (m:freePure 'a) : pure_wp 'a = 
   match m with
   | Return x -> pure_wp_return x 
@@ -33,3 +32,34 @@ let rec freePure_to_pureId #a (m:freePure a) (wp:pure_wp a) (post:a -> Type0) :
     assert (freePure_theta (k ()) `pure_wp_stronger` (freePure_theta (k ())));
     assert ((freePure_theta (k())) post);
     freePure_to_pureId (k ()) (freePure_theta (k())) post
+
+assume val state_t:Type0
+assume val state_rel : state_t -> state_t -> Type0
+
+noeq
+type freeState (a:Type) =
+| ReturnST : a -> freeState a 
+| GetST : (state_t -> freeState a) -> freeState a
+| PutST : state_t -> (unit -> freeState a) -> freeState a
+
+let state_wp a = (a -> state_t -> Type0) -> (state_t -> Type0)
+let state_wp_return (x:'a) : state_wp 'a = fun p s0 -> p x s0
+let state_wp_bind (m:state_wp 'a) (k:'a -> state_wp 'b) : state_wp 'b =
+  fun p s0 -> m (fun r s1 -> k r p s1) s0
+let state_wp_stronger (wp1 wp2:state_wp 'a) : Type0 =
+  forall p s0. wp2 p s0 ==> wp1 p s0
+
+let rec freeState_theta (m:freeState 'a) : state_wp 'a =
+  match m with
+  | ReturnST x -> state_wp_return x
+  | GetST k -> state_wp_bind (fun p s0 -> p s0 s0) (fun r -> freeState_theta (k r))
+  | PutST s1 k -> state_wp_bind (fun p s0 -> s0 `state_rel` s1 /\ p () s1) (fun r -> freeState_theta (k r))
+
+let state a = state_t -> a * state_t
+
+let rec freeState_to_state #a (m:freeState a) (wp:(state_wp a){freeState_theta m `state_wp_stronger` wp}) (post:(a -> state_t -> Type0)) (s0:state_t{wp post s0}) :
+  Tot (r:(a * state_t){post (fst r) (snd r)}) =
+  match m with
+  | ReturnST x -> (x, s0)
+  | GetST k ->  freeState_to_state (k s0) (freeState_theta (k s0)) post s0
+  | PutST s1 k -> freeState_to_state (k ()) (freeState_theta (k ())) post s1
